Logic/Predicate/FirstOrder/Deduction/Meta.lean
@@ -9,6 +9,7 @@ namespace Deduction
 open SubFormula
 variable {L : Language.{u}} [∀ k, DecidableEq (L.func k)] [∀ k, DecidableEq (L.rel k)] [L.Eq]
 variable {T : Theory L} [EqTheory T]
+variable {Δ : List (SyntacticFormula L)}
 
 def generalizeOfEq {Δ Δ' p p'}
   (hΔ : Δ.map shift = Δ') (hp : free p = p') (b : Δ' ⟹[T] p') : Δ ⟹[T] ∀' p :=
@@ -26,6 +27,99 @@ def exCasesOfEq {Δ Δ' p p' q q'}
 def useInstanceOfEq (t) {Δ p p'} (h : ⟦↦ t⟧ p = p')
   (b : Δ ⟹[T] p') : Δ ⟹[T] ∃' p :=
   useInstance t (b.cast h.symm)
+
+def weakening {Δ Γ p} (h : Δ ⊆ Γ) (b : Δ ⟹[T] p) : Γ ⟹[T] p :=
+  b.weakening' (List.cons_subset_cons _ h)
+
+protected def shift {p} (b : Δ ⟹[T] p) : (Δ.map shift) ⟹[T] shift p :=
+  b.rewrite _
+
+def absurd {p} (b : (p :: Δ) ⟹[T] ⊥) : Δ ⟹[T] ~p :=
+  (contradiction (~p) trivial b).weakening' (by simp)
+
+def splitIff {p q} (b₁ : Δ ⟹[T] p ⟶ q) (b₂ : Δ ⟹[T] q ⟶ p) : Δ ⟹[T] p ⟷ q :=
+  split b₁ b₂
+
+def modusPonensOfIffLeft {p q} (b₀ : Δ ⟹[T] p ⟷ q) (b₁ : Δ ⟹[T] p) : Δ ⟹[T] q :=
+  b₀.andLeft.modusPonens b₁
+
+def modusPonensOfIffRight {p q} (b₀ : Δ ⟹[T] p ⟷ q) (b₁ : Δ ⟹[T] q) : Δ ⟹[T] p :=
+  b₀.andRight.modusPonens b₁
+
+def iffRefl (p) : Δ ⟹[T] p ⟷ p := split (intro $ assumption $ by simp) (intro $ assumption $ by simp) 
+
+def iffReflOfEq {p q} (h : p = q) : Δ ⟹[T] p ⟷ q := by rw [h]; exact iffRefl q
+
+def iffSymm {p q} (b : Δ ⟹[T] p ⟷ q) : Δ ⟹[T] q ⟷ p :=
+  b.andRight.split b.andLeft
+
+def iffTrans {p q r} (b₁ : Δ ⟹[T] p ⟷ q) (b₂ : Δ ⟹[T] q ⟷ r) : Δ ⟹[T] p ⟷ r :=
+  split
+    (intro $ modusPonens (b₂.andLeft.weakening (by simp)) $
+      modusPonens (b₁.andLeft.weakening (by simp)) $ assumption (by simp))
+    (intro $ modusPonens (b₁.andRight.weakening (by simp)) $
+      modusPonens (b₂.andRight.weakening (by simp)) $ assumption (by simp))
+
+def iffAnd {p₁ p₂ q₁ q₂} (b₁ : Δ ⟹[T] p₁ ⟷ q₁) (b₂ : Δ ⟹[T] p₂ ⟷ q₂) : Δ ⟹[T] p₁ ⋏ p₂ ⟷ q₁ ⋏ q₂ :=
+  splitIff
+    (intro $ split
+        ((b₁.andLeft.weakening (List.subset_cons_of_subset _ $ by simp[List.subset_cons])).modusPonens $ andLeft (q := p₂) (assumption $ by simp))
+        ((b₂.andLeft.weakening (List.subset_cons_of_subset _ $ by simp[List.subset_cons])).modusPonens $ andRight (p := p₁) (assumption $ by simp)))
+    (intro $ split
+        ((b₁.andRight.weakening (List.subset_cons_of_subset _ $ by simp[List.subset_cons])).modusPonens $ andLeft (q := q₂) (assumption $ by simp))
+        ((b₂.andRight.weakening (List.subset_cons_of_subset _ $ by simp[List.subset_cons])).modusPonens $ andRight (p := q₁) (assumption $ by simp)))
+
+def iffOr {p₁ p₂ q₁ q₂} (b₁ : Δ ⟹[T] p₁ ⟷ q₁) (b₂ : Δ ⟹[T] p₂ ⟷ q₂) : Δ ⟹[T] p₁ ⋎ p₂ ⟷ q₁ ⋎ q₂ :=
+  splitIff
+    (intro $ cases (p := p₁) (q := p₂) (assumption $ by simp)
+      (orLeft $ (b₁.andLeft.weakening (List.subset_cons_of_subset _ $ by simp[List.subset_cons])).modusPonens $ assumption $ by simp)
+      (orRight $ (b₂.andLeft.weakening (List.subset_cons_of_subset _ $ by simp[List.subset_cons])).modusPonens $ assumption $ by simp))
+    (intro $ cases (p := q₁) (q := q₂) (assumption $ by simp)
+      (orLeft $ (b₁.andRight.weakening (List.subset_cons_of_subset _ $ by simp[List.subset_cons])).modusPonens $ assumption $ by simp)
+      (orRight $ (b₂.andRight.weakening (List.subset_cons_of_subset _ $ by simp[List.subset_cons])).modusPonens $ assumption $ by simp))
+
+def iffNeg {p q} (b : Δ ⟹[T] p ⟷ q) : Δ ⟹[T] ~p ⟷ ~q :=
+  splitIff
+    (intro $ absurd $ contradiction (p := p) ⊥
+      ((b.andRight.weakening (List.subset_cons_of_subset _ $ by simp)).modusPonens $ assumption $ by simp)
+      (assumption $ by simp))
+    (intro $ absurd $ contradiction (p := q) ⊥
+      ((b.andLeft.weakening (List.subset_cons_of_subset _ $ by simp)).modusPonens $ assumption $ by simp)
+      (assumption $ by simp))
+
+def iffAll {p q} (b : Δ.map shift ⟹[T] free p ⟷ free q) : Δ ⟹[T] ∀' p ⟷ ∀' q :=
+  splitIff
+    (intro $ generalize $ (b.andLeft.weakening $ by simp).modusPonens $
+      (specialize &0 (p := shift p) $ assumption $ by simp).cast (by simp))
+    (intro $ generalize $ (b.andRight.weakening $ by simp).modusPonens $
+      (specialize &0 (p := shift q) $ assumption $ by simp).cast (by simp))
+
+def iffEx {p q} (b : Δ.map shift ⟹[T] free p ⟷ free q) : Δ ⟹[T] ∃' p ⟷ ∃' q :=
+  splitIff
+    (intro $ exCases (p := p) (assumption $ by simp) $ (useInstance &0 (p := shift q) $
+      ((b.andLeft.weakening (List.subset_cons_of_subset _ $ by simp)).modusPonens $ assumption $ by simp).cast (by simp)).cast (by simp))
+    (intro $ exCases (p := q) (assumption $ by simp) $ (useInstance &0 (p := shift p) $
+      ((b.andRight.weakening (List.subset_cons_of_subset _ $ by simp)).modusPonens $ assumption $ by simp).cast (by simp)).cast (by simp))
+
+inductive IffFormula : (p₀ q₀ : SyntacticFormula L) → SyntacticFormula L → SyntacticFormula L → Type u
+  | intro {p₀ q₀} : IffFormula p₀ q₀ p₀ q₀
+  | refl {p₀ q₀} : (p : SyntacticFormula L) → IffFormula p₀ q₀ p p
+  | and {p₀ q₀ p₁ p₂ q₁ q₂} : IffFormula p₀ q₀ p₁ q₁ → IffFormula p₀ q₀ p₂ q₂ → IffFormula p₀ q₀ (p₁ ⋏ p₂) (q₁ ⋏ q₂)
+  | or {p₀ q₀ p₁ p₂ q₁ q₂} : IffFormula p₀ q₀ p₁ q₁ → IffFormula p₀ q₀ p₂ q₂ → IffFormula p₀ q₀ (p₁ ⋎ p₂) (q₁ ⋎ q₂)
+  | all {p₀ q₀} {p q : SyntacticSubFormula L 1} : IffFormula (shift p₀) (shift q₀) (free p) (free q) → IffFormula p₀ q₀ (∀' p) (∀' q)
+  | ex {p₀ q₀} {p q : SyntacticSubFormula L 1} : IffFormula (shift p₀) (shift q₀) (free p) (free q) → IffFormula p₀ q₀ (∃' p) (∃' q)
+
+def iffOfIffFormula {p₀ q₀} :
+    {p q : SyntacticFormula L} → IffFormula p₀ q₀ p q → {Δ : List (SyntacticFormula L)} → (Δ ⟹[T] p₀ ⟷ q₀) → (Δ ⟹[T] p ⟷ q)
+  | _, _, IffFormula.intro,     _, b => b
+  | _, _, IffFormula.refl p,    Δ, _ => iffRefl _
+  | _, _, IffFormula.and h₁ h₂, Δ, b => iffAnd (iffOfIffFormula h₁ b) (iffOfIffFormula h₂ b)
+  | _, _, IffFormula.or h₁ h₂,  Δ, b => iffOr (iffOfIffFormula h₁ b) (iffOfIffFormula h₂ b)
+  | _, _, IffFormula.all h,     Δ, b => (iffOfIffFormula h (b.shift.cast $ by simp)).iffAll
+  | _, _, IffFormula.ex h,      Δ, b => (iffOfIffFormula h (b.shift.cast $ by simp)).iffEx
+
+def eqReflOfEq {t₁ t₂ : SyntacticTerm L} (h : t₁ = t₂) :
+    Δ ⟹[T] “ᵀ!t₁ = ᵀ!t₂” := by rw[h]; exact eqRefl _
 
 end Deduction
 
@@ -45,6 +139,19 @@ def generalizeOfEqQ (Δ Δ' : Q(List (SyntacticFormula $L))) (p : Q(SyntacticSub
   (hΔ : Q(($Δ).map shift = $Δ')) (hp : Q(free $p = $p')) (b : Q($Δ' ⟹[$T] $p')) : Q($Δ ⟹[$T] ∀' $p) :=
   q(Deduction.generalizeOfEq $hΔ $hp $b)
 
+def exCasesOfEqQ (Δ Δ' : Q(List (SyntacticFormula $L)))
+  (p : Q(SyntacticSubFormula $L 1)) (p' : Q(SyntacticFormula $L))
+  (q q' : Q(SyntacticFormula $L))
+  (hΔ : Q(($Δ).map shift = $Δ')) (hp : Q(free $p = $p')) (hq : Q(shift $q = $q'))
+  (b₀ : Q($Δ ⟹[$T] ∃' $p)) (b₁ : Q(($p' :: $Δ') ⟹[$T] $q')) : Q($Δ ⟹[$T] $q) :=
+  q(Deduction.exCasesOfEq $hΔ $hp $hq $b₀ $b₁)
+
+def eqReflOfEqQ (Δ : Q(List (SyntacticFormula $L))) (t₁ t₂ : Q(SyntacticTerm $L)) (h : Q($t₁ = $t₂)) :
+    Q($Δ ⟹[$T] SubFormula.rel Language.Eq.eq ![$t₁, $t₂]) := q(Deduction.eqReflOfEq $h)
+
+def iffReflOfEqQ (Δ : Q(List (SyntacticFormula $L))) (p₁ p₂ : Q(SyntacticFormula $L)) (h : Q($p₁ = $p₂)) :
+    Q($Δ ⟹[$T] $p₁ ⟷ $p₂) := q(Deduction.iffReflOfEq $h)
+
 end DeductionQ
 
 section Syntax
@@ -52,9 +159,9 @@ variable (L : Q(Language.{u})) (n : Q(ℕ))
 open SubTerm
 
 -- TODO
-partial def subTermSyntaxToExpr : Syntax → TermElabM Q(SyntacticSubTerm $L $n)
-  | `(subterm| ($s)) => subTermSyntaxToExpr s
-  | `(subterm| !$t:term) =>
+partial def subTermSyntaxToExpr (n : Q(ℕ)) : Syntax → TermElabM Q(SyntacticSubTerm $L $n)
+  | `(subterm| ($s)) => subTermSyntaxToExpr n s
+  | `(subterm| ᵀ!$t:term) =>
     Term.elabTerm t (return q(SyntacticSubTerm $L $n))
   | `(subterm| $n:num) => do
     let en ← Term.elabTerm n (return q(ℕ))
@@ -74,91 +181,114 @@ partial def subTermSyntaxToExpr : Syntax → TermElabM Q(SyntacticSubTerm $L $n)
     let ex : Q(ℕ) ← Term.elabTerm x (return q(ℕ))
     return q(&$ex)
   | `(subterm| $t₁:subterm + $t₂:subterm) => do
-    let et₁ ← subTermSyntaxToExpr t₁
-    let et₂ ← subTermSyntaxToExpr t₂
+    let et₁ ← subTermSyntaxToExpr n t₁
+    let et₂ ← subTermSyntaxToExpr n t₂
     let (_ : Q(Language.Add $L)) ← synthInstanceQ q(Language.Add $L)
     return q(SubTerm.func Language.Add.add ![$et₁, $et₂])
   | `(subterm| $t₁:subterm * $t₂:subterm) => do
-    let et₁ ← subTermSyntaxToExpr t₁
-    let et₂ ← subTermSyntaxToExpr t₂
+    let et₁ ← subTermSyntaxToExpr n t₁
+    let et₂ ← subTermSyntaxToExpr n t₂
     let (_ : Q(Language.Mul $L)) ← synthInstanceQ q(Language.Mul $L)
     return q(SubTerm.func Language.Mul.mul ![$et₁, $et₂])
   | `(subterm| $t₁:subterm ^ $t₂:subterm) => do
-    let et₁ ← subTermSyntaxToExpr t₁
-    let et₂ ← subTermSyntaxToExpr t₂
+    let et₁ ← subTermSyntaxToExpr n t₁
+    let et₂ ← subTermSyntaxToExpr n t₂
     let (_ : Q(Language.Pow $L)) ← synthInstanceQ q(Language.Pow $L)
     return q(SubTerm.func Language.Pow.pow ![$et₁, $et₂])
+  | `(subterm| $t ᵀ⟦$v:subterm,*⟧) => do
+    let e0 : Q(Fin 0 → SyntacticSubTerm $L $n) := q(![])
+    let (k, ev) ← v.getElems.foldlM (β := ℕ × Expr)
+      (init := (0, (e0 : Expr)))
+      (fun (k, e) s => do
+        let ih : Q(Fin $k → SyntacticSubTerm $L $n) := e
+        let es : Q(SyntacticSubTerm $L $n) ← subTermSyntaxToExpr n s
+        let e : Q(Fin ($k + 1) → SyntacticSubTerm $L $n) := q($es :> $ih) 
+        return (k + 1, e))
+    let ev : Q(Fin $k → SyntacticSubTerm $L $n) := ev
+    let et ← subTermSyntaxToExpr q($k) t
+    return q(substs $ev $et)
   | _                    => throwUnsupportedSyntax
   
-
 -- TODO
-partial def subFormulaSyntaxToExpr : (n : Q(ℕ)) → Syntax → TermElabM Q(SyntacticSubFormula $L $n)
-  | n, `(subformula| ($p)) => subFormulaSyntaxToExpr n p
-  | n, `(subformula| !$t:term)  =>
+partial def subFormulaSyntaxToExpr (n : Q(ℕ)) : Syntax → TermElabM Q(SyntacticSubFormula $L $n)
+  | `(subformula| ($p)) => subFormulaSyntaxToExpr n p
+  | `(subformula| !$t:term)  =>
     Term.elabTerm t (return q(SyntacticSubFormula $L $n))
 
-  | n, `(subformula| $t₁:subterm = $t₂:subterm) => do
+  | `(subformula| $t₁:subterm = $t₂:subterm) => do
     let et₁ ← subTermSyntaxToExpr L n t₁
     let et₂ ← subTermSyntaxToExpr L n t₂
     let (_ : Q(Language.Eq $L)) ← synthInstanceQ q(Language.Eq $L)
     let e : Expr := q(SubFormula.rel Language.Eq.eq ![$et₁, $et₂])
     return e
-  | n, `(subformula| $t₁:subterm ≠ $t₂:subterm) => do
+  | `(subformula| $t₁:subterm ≠ $t₂:subterm) => do
     let et₁ ← subTermSyntaxToExpr L n t₁
     let et₂ ← subTermSyntaxToExpr L n t₂
     let (_ : Q(Language.Eq $L)) ← synthInstanceQ q(Language.Eq $L)
     let e : Expr := q(SubFormula.nrel Language.Eq.eq ![$et₁, $et₂])
     return e
 
-  | n, `(subformula| $t₁:subterm < $t₂:subterm) => do
+  | `(subformula| $t₁:subterm < $t₂:subterm) => do
     let et₁ ← subTermSyntaxToExpr L n t₁
     let et₂ ← subTermSyntaxToExpr L n t₂
     let (_ : Q(Language.Lt $L)) ← synthInstanceQ q(Language.Lt $L)
     let e : Expr := q(SubFormula.rel Language.Lt.lt ![$et₁, $et₂])
     return e
-  | n, `(subformula| $t₁:subterm ≮ $t₂:subterm) => do
+  | `(subformula| $t₁:subterm ≮ $t₂:subterm) => do
     let et₁ ← subTermSyntaxToExpr L n t₁
     let et₂ ← subTermSyntaxToExpr L n t₂
     let (_ : Q(Language.Lt $L)) ← synthInstanceQ q(Language.Lt $L)
     let e : Expr := q(SubFormula.nrel Language.Lt.lt ![$et₁, $et₂])
     return e
 
-  | _, `(subformula| ⊤)       => return q(⊤)
-  | _, `(subformula| ⊥)       => return q(⊥)
-  | n, `(subformula| $p ∧ $q) => do
+  | `(subformula| ⊤)       => return q(⊤)
+  | `(subformula| ⊥)       => return q(⊥)
+  | `(subformula| $p ∧ $q) => do
     let ep ← subFormulaSyntaxToExpr n p
     let eq ← subFormulaSyntaxToExpr n q
     let epandeq : Expr := q($ep ⋏ $eq)
     return epandeq
-  | n, `(subformula| $p ∨ $q) => do
+  | `(subformula| $p ∨ $q) => do
     let ep ← subFormulaSyntaxToExpr n p
     let eq ← subFormulaSyntaxToExpr n q
     let eporeq : Expr := q($ep ⋏ $eq)
     return eporeq
-  | n, `(subformula| ∀ $p)     => do
+  | `(subformula| ∀ $p)     => do
     let ep ← subFormulaSyntaxToExpr q($n + 1) p
     let allep : Expr := q(∀' $ep)
     return allep
-  | n, `(subformula| ∃ $p)     => do
+  | `(subformula| ∃ $p)     => do
     let ep ← subFormulaSyntaxToExpr q($n + 1) p
     let exep : Expr := q(∃' $ep)
     return exep
 
-  | n, `(subformula| ¬$p)     => do
+  | `(subformula| ¬$p)     => do
     let ep ← subFormulaSyntaxToExpr n p
     have nep : Expr := q(~$ep)
     return nep
-  | n, `(subformula| $p → $q) => do
+  | `(subformula| $p → $q) => do
     let ep ← subFormulaSyntaxToExpr n p
     let eq ← subFormulaSyntaxToExpr n q
     let eptoeq : Expr := q($ep ⟶ $eq)
     return eptoeq
-  | n, `(subformula| $p ↔ $q) => do
+  | `(subformula| $p ↔ $q) => do
     let ep ← subFormulaSyntaxToExpr n p
     let eq ← subFormulaSyntaxToExpr n q
     let epiffeq : Expr := q($ep ⟷ $eq)
-    return epiffeq  
-  | _, _                   => throwUnsupportedSyntax
+    return epiffeq
+  | `(subformula| $p ⟦$v:subterm,*⟧) => do
+    let e0 : Q(Fin 0 → SyntacticSubTerm $L $n) := q(![])
+    let (k, ev) ← v.getElems.foldlM (β := ℕ × Expr)
+      (init := (0, (e0 : Expr)))
+      (fun (k, e) s => do
+        let ih : Q(Fin $k → SyntacticSubTerm $L $n) := e
+        let es : Q(SyntacticSubTerm $L $n) ← subTermSyntaxToExpr L n s
+        let e : Q(Fin ($k + 1) → SyntacticSubTerm $L $n) := q($es :> $ih) 
+        return (k + 1, e))
+    let ev : Q(Fin $k → SyntacticSubTerm $L $n) := ev
+    let ep ← subFormulaSyntaxToExpr q($k) p
+    return q(SubFormula.substs $ev $ep)
+  | _                   => throwUnsupportedSyntax
 
 partial def formulaSyntaxToExpr (s : Syntax) : TermElabM Q(SyntacticFormula $L) :=
   subFormulaSyntaxToExpr L q(0) s
@@ -172,18 +302,23 @@ inductive DeductionCode (L : Q(Language.{u})) : Type
   | trivial       : DeductionCode L
   | explode       : DeductionCode L → DeductionCode L
   | intro         : DeductionCode L → DeductionCode L
-  | modusPonens           : Q(SyntacticFormula $L) → DeductionCode L → DeductionCode L → DeductionCode L  
+  | modusPonens   : Q(SyntacticFormula $L) → DeductionCode L → DeductionCode L → DeductionCode L  
   | split         : DeductionCode L → DeductionCode L → DeductionCode L
-  -- TODO
+  | andLeft       : Q(SyntacticFormula $L) → DeductionCode L → DeductionCode L
+  | andRight      : Q(SyntacticFormula $L) → DeductionCode L → DeductionCode L
+  | orLeft        : DeductionCode L → DeductionCode L
+  | orRight       : DeductionCode L → DeductionCode L
   | cases         : (e₁ e₂ : Q(SyntacticFormula $L)) → DeductionCode L → DeductionCode L → DeductionCode L → DeductionCode L
   | generalize    : DeductionCode L → DeductionCode L
-  -- TODO
-  | exCases       : Q(SyntacticFormula $L) → DeductionCode L → DeductionCode L → DeductionCode L
+  | specialize    : Q(SyntacticTerm $L) → DeductionCode L → DeductionCode L
+  | useInstance   : Q(SyntacticTerm $L) → DeductionCode L → DeductionCode L
+  | exCases       : Q(SyntacticSubFormula $L 1) → DeductionCode L → DeductionCode L → DeductionCode L
   | eqRefl        : DeductionCode L
   | eqSymm        : DeductionCode L → DeductionCode L
   | eqTrans       : Q(SyntacticFormula $L) → DeductionCode L → DeductionCode L → DeductionCode L
   | rewriteEq     : (e₁ e₂ : Q(SyntacticTerm $L)) → DeductionCode L → DeductionCode L → DeductionCode L
   | since         : Syntax → DeductionCode L
+  | showState     : DeductionCode L → DeductionCode L
   | missing       : DeductionCode L
   -- TODO
 
@@ -199,14 +334,21 @@ def toStr : DeductionCode L → String
   | intro c               => "intro\n" ++ c.toStr
   | modusPonens _ c₁ c₂   => "have: {\n" ++ c₁.toStr ++ "\n}\nand: {\n" ++ c₂.toStr ++ "\n}"
   | split c₁ c₂           => "∧ split: {\n" ++ c₁.toStr ++ "\n}\nand: {\n" ++ c₂.toStr ++ "\n}"
+  | andLeft _ c           => "∧ left\n" ++ c.toStr
+  | andRight _ c          => "∧ right\n" ++ c.toStr
+  | orLeft c              => "∨ left\n" ++ c.toStr
+  | orRight c             => "∨ right\n" ++ c.toStr
   | cases _ _ c₀ c₁ c₂    => "∨ split: {\n" ++ c₀.toStr ++ "\n}\nor left: {\n" ++ c₁.toStr ++ "\n}\nor right: {\n" ++ c₂.toStr ++ "\n}"
   | generalize c          => "generalize\n" ++ c.toStr
+  | specialize _ c        => "specialize\n" ++ c.toStr
+  | useInstance _ c       => "use\n" ++ c.toStr
   | exCases _ c₀ c₁       => "∃ cases: {\n" ++ c₀.toStr ++ "\n}\n" ++ c₁.toStr
   | eqRefl                => "refl"
   | eqSymm c              => "symmetry" ++ c.toStr
   | eqTrans _ c₁ c₂       => "trans: {\n" ++ c₁.toStr ++ "\n}\n and: {\n" ++ c₂.toStr ++ "\n}"
   | rewriteEq _ _ c₁ c₂   => "rewrite: {\n" ++ c₁.toStr ++ "\n}\n" ++ c₂.toStr
   | since _               => "since"
+  | showState c           => c.toStr
   | missing               => "?"
 
 instance : Repr (DeductionCode L) := ⟨fun b _ => b.toStr L⟩
@@ -216,23 +358,31 @@ instance : ToString (DeductionCode L) := ⟨toStr L⟩
 variable (dfunc : Q(∀ k, DecidableEq (($L).func k))) (drel : Q(∀ k, DecidableEq (($L).rel k))) (lEq : Q(Language.Eq $L)) 
 variable (T : Q(Theory $L)) (eqTh : Q(EqTheory $T))
 
+
+def display (E : List Q(SyntacticFormula $L)) (e : Q(SyntacticFormula $L)) : MetaM Unit := do
+  -- logInfo m!"Language: {L}\nTheory: {T}"
+  let (_, m) := E.foldr (fun e (s, m) => (s + 1, m ++ m!"{s+1}:    {e}\n")) (0, m! "")
+  logInfo (m ++ m!"⊢\n0:    {e}")
+
+#check Deduction.exCases
+
 def run : (c : DeductionCode L) → (G : List Q(SyntacticFormula $L)) → (e : Q(SyntacticFormula $L)) →
     TermElabM Q($(Qq.toQList (u := u) G) ⟹[$T] $e)
   | assumption,            E, e  => do
-    let some eh ← Qq.memQList? (u := u) e E | throwError m!"failed to prove {e} ∈ {E}" --el eVerum
+    let some eh ← Qq.memQList? (u := u) e E | do display L E e; throwError m!"failed to prove {e} ∈ {E}" --el eVerum
     return DeductionQ.assumptionQ L dfunc drel lEq T (Qq.toQList (u := u) E) e eh
   | trans e₁ c₁ c₂,        E, e₂ => do
     let b₁ ← c₁.run E e₁
     let b₂ ← c₂.run (e₁ :: E) e₂
     return q(Deduction.trans $b₁ $b₂)
-  | contradiction e c₁ c₂, E, _  => do
-    let b₁ ← c₁.run E e
-    let b₂ ← c₂.run E q(~$e)
-    return q(Deduction.contradiction $e $b₁ $b₂)
+  | contradiction e₀ c₁ c₂, E, e₁  => do
+    let b₁ ← c₁.run E e₀
+    let b₂ ← c₂.run E q(~$e₀)
+    return q(Deduction.contradiction $e₁ $b₁ $b₂)
   | trivial,               _, e  => do
     match e with
     | ~q(⊤) => return q(Deduction.trivial)
-    | _ => throwError "incorrect structure"
+    | _ => throwError "incorrect structure: {e} should be ⊤"
   | explode c,             E, _  => do
     let b ← c.run E q(⊥)
     return q(Deduction.explode $b)
@@ -241,7 +391,7 @@ def run : (c : DeductionCode L) → (G : List Q(SyntacticFormula $L)) → (e : Q
     | ~q($e₁ ⟶ $e₂) =>
       let b ← c.run (e₁ :: E) e₂
       return q(Deduction.intro $b)
-    | _ => throwError "incorrect structure"
+    | _ => throwError "incorrect structure: {e} should be _ → _"
   | modusPonens e₁ c₁ c₂,  E, e₂ => do
     let b₁ ← c₁.run E q($e₁ ⟶ $e₂)
     let b₂ ← c₂.run E e₁
@@ -252,7 +402,29 @@ def run : (c : DeductionCode L) → (G : List Q(SyntacticFormula $L)) → (e : Q
       let b₁ ← c₁.run E e₁
       let b₂ ← c₂.run E e₂
       return q(Deduction.split $b₁ $b₂)
-    | _ => throwError "incorrect structure"
+    | ~q($e₁ ⟷ $e₂) =>
+      let b₁ ← c₁.run E q($e₁ ⟶ $e₂)
+      let b₂ ← c₂.run E q($e₂ ⟶ $e₁)
+      return q(Deduction.splitIff $b₁ $b₂)
+    | _ => throwError "incorrect structure: {e} should be _ ⋏ _ or _ ⟷ _"
+  | andLeft e₁ c,           E, e₂  => do
+      let b ← c.run E q($e₂ ⋏ $e₁)
+      return q(Deduction.andLeft $b)
+  | andRight e₁ c,           E, e₂  => do
+      let b ← c.run E q($e₁ ⋏ $e₂)
+      return q(Deduction.andRight $b)
+  | orLeft c,               E, e  => do
+    match e with
+    | ~q($e₁ ⋎ $e₂) =>
+      let b ← c.run E e₁
+      return q(Deduction.orLeft $b)
+    | _ => throwError "incorrect structure: {e} should be _ ⋎ _"
+  | orRight c,               E, e  => do
+    match e with
+    | ~q($e₁ ⋎ $e₂) =>
+      let b ← c.run E e₂
+      return q(Deduction.orRight $b)
+    | _ => throwError "incorrect structure: {e} should be _ ⋎ _"
   | cases e₁ e₂ c₀ c₁ c₂,  E, e  => do
     let b₀ ← c₀.run E q($e₁ ⋎ $e₂)
     let b₁ ← c₁.run (e₁ :: E) e
@@ -266,27 +438,45 @@ def run : (c : DeductionCode L) → (G : List Q(SyntacticFormula $L)) → (e : Q
       let b ← c.run sE fe
       return DeductionQ.generalizeOfEqQ L dfunc drel lEq T
         (Qq.toQList (u := u) E) (Qq.toQList (u := u) sE) e fe sEe fee b
-    | _ => throwError "incorrect structure: generalize"
+    | _ => throwError "incorrect structure: {e} should be ∀ _"
+  | exCases e c₀ c₁,          E, i => do
+    let ⟨fe, fee⟩ ← SubFormula.Meta.resultFree (L := L) (n := q(0)) e
+    let ⟨si, sie⟩ ← SubFormula.Meta.resultShift (L := L) (n := q(0)) i
+    let ⟨sE, sEe⟩ ← SubFormula.Meta.resultShift₀List E
+    let b₀ ← c₀.run E q(∃' $e)
+    let b₁ ← c₁.run (fe :: sE) si
+    return DeductionQ.exCasesOfEqQ L dfunc drel lEq T
+      (Qq.toQList (u := u) E) (Qq.toQList (u := u) sE) e fe i si sEe fee sie b₀ b₁
+  | eqRefl, E, i => do
+    match i with
+    | ~q(SubFormula.rel Language.Eq.eq ![$i₁, $i₂]) =>
+      let ⟨i₁', ie₁⟩ ← SubTerm.Meta.result (L := L) (n := q(0)) SubTerm.Meta.NumeralUnfoldOption.all i₁
+      let ⟨i₂', ie₂⟩ ← SubTerm.Meta.result (L := L) (n := q(0)) SubTerm.Meta.NumeralUnfoldOption.all i₂
+      if (← isDefEq i₁' i₂') then
+        let eqn : Q($i₁' = $i₂') := (q(@rfl (SyntacticTerm $L) $i₁') : Expr)
+        let eqn : Q($i₁ = $i₂) := q(Eq.trans $ie₁ $ Eq.trans $eqn $ Eq.symm $ie₂)
+        return DeductionQ.eqReflOfEqQ L dfunc drel lEq T (Qq.toQList (u := u) E) i₁ i₂ eqn
+      else throwError "term should be equal: {i₁}, {i₂}"
+    | ~q($p₁ ⟷ $p₂) =>
+      let ⟨p₁', pe₁⟩ ← SubFormula.Meta.result (L := L) (n := q(0)) SubTerm.Meta.NumeralUnfoldOption.all SubFormula.Meta.unfoldAll p₁
+      let ⟨p₂', pe₂⟩ ← SubFormula.Meta.result (L := L) (n := q(0)) SubTerm.Meta.NumeralUnfoldOption.all SubFormula.Meta.unfoldAll p₂
+      if (← isDefEq p₁' p₂') then
+        let eqn : Q($p₁' = $p₂') := (q(@rfl (SyntacticFormula $L) $p₁') : Expr)
+        let eqn : Q($p₁ = $p₂) := q(Eq.trans $pe₁ $ Eq.trans $eqn $ Eq.symm $pe₂)
+        return DeductionQ.iffReflOfEqQ L dfunc drel lEq T (Qq.toQList (u := u) E) p₁ p₂ eqn
+      else throwError "term should be equal: {p₁}, {p₂}"
+    | _ => throwError "incorrect structure: {i} should be _ = _ or _ ↔ _"
   | since s, E, e               => do
     Term.elabTerm s (return q($(Qq.toQList (u := u) E) ⟹[$T] $e))
+  | showState c,          E, e  => do
+    display L E e
+    let b ← c.run E e
+    return q($b)
   | _, E, e               => do
-    throwError m!"proof is missing:\n  {E}\n  ⊢\n  {e}"
-
-elab "test" : term => do
-  have L : Q(Language.{0}) := q(Language.oring)
-  let c : DeductionCode L := intro (trans q(⊤) trivial assumption)
-  let dfunc ← synthInstanceQ q(∀ k, DecidableEq (($L).func k))
-  let drel  ← synthInstanceQ q(∀ k, DecidableEq (($L).rel k))
-  let lEq : Q(Language.Eq $L)   ← synthInstanceQ q(Language.Eq $L)
-  let T := q(@Theory.Eq $L $lEq)
-  let b ← c.run L dfunc drel lEq T [q(⊥)] q(⊤ ⟶ ⊤)
-  logInfo m! "{b}"
-  return b
-
-#eval test
+    display L E e
+    throwError m!"proof is missing" 
 
 end DeductionCode
-
 
 open Lean.Parser
 
@@ -314,14 +504,29 @@ syntax (name := notationTrivial) "trivial" : proofElem
 
 syntax (name := notationIntro) "intro" : proofElem
 
+syntax (name := notationModusPonens) "suffices" subformula optProofBlock : proofElem
+
 syntax (name := notationSplit)"split" optProofBlock optProofBlock : proofElem
+
+syntax (name := notationAndLeft) "andl" subformula optProofBlock : proofElem
+
+syntax (name := notationAndRight) "andr" subformula optProofBlock : proofElem
+
+syntax (name := notationOrLeft) "left" optProofBlock : proofElem
+
+syntax (name := notationOrRight) "right" optProofBlock : proofElem
 
 syntax (name := notationCases) "cases " subformula " or " subformula optProofBlock proofBlock proofBlock : proofElem
 
 syntax (name := notationGeneralize) "generalize" : proofElem
 
+syntax (name := notationExCases) "invoke " subformula optProofBlock : proofElem
+
+syntax (name := notationEqRefl) "rfl" : proofElem
+
 syntax (name := notationSince) "since" term : proofElem
 
+syntax (name := notationShowState) "!" : proofElem
 
 syntax (name := notationMissing) "?" : proofElem
 
@@ -366,13 +571,36 @@ partial def seqToCode (L : Q(Language.{u})) : List Syntax → TermElabM (Deducti
       --logInfo f!"seqElem : {seqElem}"
       let c ← seqToCode L seqElems
       return DeductionCode.intro c
-    -- TODO: else if k == ``notationModusPonens then
+    else if k == ``notationModusPonens then
+      let e ← formulaSyntaxToExpr L seqElem[1]
+      let s := getSeqOfOptProofBlock seqElem[2]
+      let c₀ := if s.isMissing then DeductionCode.assumption else ← seqToCode L (getSeqElems <| s)
+      let c₁ ← seqToCode L seqElems
+      return DeductionCode.modusPonens e c₀ c₁
     else if k == ``notationSplit then
       let s₁ := getSeqOfOptProofBlock seqElem[1] 
       let s₂ := getSeqOfOptProofBlock seqElem[2]
       let c₁ := if s₁.isMissing then DeductionCode.assumption else ← seqToCode L (getSeqElems <| s₁)
       let c₂ := if s₂.isMissing then DeductionCode.assumption else ← seqToCode L (getSeqElems <| s₂)
       return DeductionCode.split c₁ c₂
+    else if k == ``notationAndLeft then
+      let e ← formulaSyntaxToExpr L seqElem[1]
+      let s := getSeqOfOptProofBlock seqElem[2] 
+      let c := if s.isMissing then DeductionCode.assumption else ← seqToCode L (getSeqElems <| s)
+      return DeductionCode.andLeft e c
+    else if k == ``notationAndRight then
+      let e ← formulaSyntaxToExpr L seqElem[1]
+      let s := getSeqOfOptProofBlock seqElem[2] 
+      let c := if s.isMissing then DeductionCode.assumption else ← seqToCode L (getSeqElems <| s)
+      return DeductionCode.andRight e c
+    else if k == ``notationOrLeft then
+      let s := getSeqOfOptProofBlock seqElem[1] 
+      let c := if s.isMissing then DeductionCode.assumption else ← seqToCode L (getSeqElems <| s)
+      return DeductionCode.orLeft c
+    else if k == ``notationOrRight then
+      let s := getSeqOfOptProofBlock seqElem[1] 
+      let c := if s.isMissing then DeductionCode.assumption else ← seqToCode L (getSeqElems <| s)
+      return DeductionCode.orRight c
     else if k == ``notationCases then
       let s₀ := getSeqOfOptProofBlock seqElem[4] 
       let s₁ := getSeqOfOptProofBlock seqElem[5]
@@ -385,15 +613,24 @@ partial def seqToCode (L : Q(Language.{u})) : List Syntax → TermElabM (Deducti
       return DeductionCode.cases e₁ e₂ c₀ c₁ c₂
     else if k == ``notationGeneralize then
       let c ← seqToCode L seqElems
-      return DeductionCode.generalize c
-      
-    -- TODO: else if k == ``notationExCases then
+      return DeductionCode.generalize c      
+    else if k == ``notationExCases then
+      let e ← subFormulaSyntaxToExpr L q(1) seqElem[1]
+      let s := getSeqOfOptProofBlock seqElem[2] 
+      let c₀ := if s.isMissing then DeductionCode.assumption else ← seqToCode L (getSeqElems <| s)
+      let c₁ ← seqToCode L seqElems
+      return DeductionCode.exCases e c₀ c₁
+    else if k == ``notationEqRefl then
+      return DeductionCode.eqRefl
     -- TODO: else if k == ``notationEqRefl then
     -- TODO: else if k == ``notationEqSymm then
     -- TODO: else if k == ``notationEqTrans then
     -- TODO: else if k == ``notationRewriteEq then
     else if k == ``notationSince then
       return DeductionCode.since seqElem[1]
+    else if k == ``notationShowState then
+      let c ← seqToCode L seqElems
+      return DeductionCode.showState c
     else if k == ``notationMissing then
       return DeductionCode.missing
     else throwError f!"no match: {k}"
@@ -427,11 +664,16 @@ example : [“0 = &1”] ⟹[T] “⊤ ∧ (2 < 3 → 0 = &1)” :=
     @ trivial
     @ intro assumption
   □
- 
-example : [“0 = &1”] ⟹[T] “⊤ ∧ (2 < 3 → 0 = &1)” :=
+
+example : [“0 = 1”, “0 ≠ 1”] ⟹[T] “⊥” :=
   proof.
-    have ⊤
-    · trivial
+    contradiction 0 = 1
+  □
+
+example : [“0 = &1”] ⟹[T]
+  “⊤ ∧ (2 < 3 → 0 = &1)” :=
+  proof.
+    have ⊤ · trivial
     split
     @ since
       proof.
@@ -442,14 +684,50 @@ example : [“0 = &1”] ⟹[T] “⊤ ∧ (2 < 3 → 0 = &1)” :=
   □
 
 -- generalize
-example : [“0 = &1”] ⟹[T] “∀ ∀ ∀ ((#0 = 0 ∨ #1 ≠ 0 ∨ #2 = 0) → ⊤)” :=
+example : [“0 = &1”, “3 < &6 + &7”] ⟹[T] “∀ ∀ ∀ ((#0 = 0 ∨ #1 ≠ 0 ∨ #2 = 0) → ⊤)” :=
   proof.
+    generalize 
+    generalize 
     generalize
-    generalize
-    generalize
-    intro
+    intro 
     trivial
   □
+
+example (t : SyntacticSubTerm L 1) :
+    [“&0 < 1 → &0 = 0”, “&0 < 1”] ⟹[T] “&0 = 0” :=
+  proof.
+    suffices &0 < 1
+    assumption
+  □
+
+example (t : SyntacticSubTerm L 1) :
+    [“&0 < 1 → &0 = 0”, “&0 < 1”] ⟹[T] “&0 = 0 ∨ 0 < 2” :=
+  proof.
+    have &0 = 0
+    · suffices &0 < 1
+        assumption
+    left
+  □
+
+example :
+    [“∃ #0 < &1”] ⟹[T] “⊤” :=
+  proof.
+    invoke #0 < &1
+    trivial
+  □
+
+example :
+    [] ⟹[T] “2 = 1 + 1” :=
+  proof.
+    rfl
+  □
+
+example :
+    [] ⟹[T] “2 = 1 + 1 ↔ 1 + 1 = 2” :=
+  proof.
+    rfl
+  □
+
 end
 
 end Meta
